good progress

TestVectors/runtimes/net/tests/Extern/GetTestDirectoryExtern.cs
@@ -1,0 +1,9 @@
+using byteseq = Dafny.Sequence<byte>;
+
+namespace TestWrappedESDKMain_Compile {
+  public partial class __default {
+    public static Dafny.ISequence<char> GetTestVectorExecutionDirectory() {
+        return byteseq.FromString("");
+    }
+  }
+}
