TestVectors/dafny/ESDK/src/VectorsComposition/AllEsdkV4NoReqEc.dfy
@@ -1,0 +1,165 @@
+// Copyright Amazon.com Inc. or its affiliates. All Rights Reserved.
+// SPDX-License-Identifier: Apache-2.0
+
+include "../LibraryIndex.dfy"
+
+module {:options "/functionSyntax:4" } AllEsdkV4NoReqEc {
+  import Types = AwsCryptographyEncryptionSdkTypes
+  import mplTypes = AwsCryptographyMaterialProvidersTypes
+  import EncryptionSdk
+  import MaterialProviders
+  import opened CompleteVectors
+  import opened KeyDescription
+  import opened Wrappers
+  import opened StandardLibrary.UInt
+  import HexStrings
+  import opened JSON.Values
+  import JSONHelpers
+  import EsdkManifestOptions
+  import EsdkTestVectors
+  
+  import AllHierarchy
+  import AllKms
+  import AllKmsMrkAware
+  import AllKmsMrkAwareDiscovery
+  import AllKmsRsa
+  import AllKmsEcdh
+  import AllRawAES
+  import AllRawRSA
+  import AllRawECDH
+  import AllDefaultCmm
+  import AllRequiredEncryptionContextCmm
+  import AllMulti
+
+  import UUID
+  import UTF8
+  import JSON.API
+  import SortedSets
+  import FileIO
+  
+  // This is a HACK!
+  // This is *ONLY* because this is wrapping the MPL
+  import AlgorithmSuites
+  
+  const frameSize: int64 := 512
+
+  const AllPositiveKeyDescriptions
+  := {}
+      + AllHierarchy.KeyDescriptions
+      + AllKms.KeyDescriptions
+      + AllKmsMrkAware.KeyDescriptions
+      + AllKmsMrkAwareDiscovery.KeyDescriptions
+      + AllKmsRsa.KeyDescriptions
+      + AllRawAES.KeyDescriptions
+      + AllRawRSA.KeyDescriptions
+      + AllMulti.KeyDescriptions
+
+  // All these tests will use a defualt CMM no ECDH
+  const AllPostiveKeyringTestsNoDBESuiteNoReqECNoEcdh :=
+  set
+    postiveKeyDescription <- AllPositiveKeyDescriptions,
+    algorithmSuite <-
+      AllAlgorithmSuites.ESDKAlgorithmSuites
+    ::
+      EsdkTestVectors.PositiveEncryptTestVectorV4(
+        encryptDescriptions := [postiveKeyDescription],
+        decryptDescriptions := [postiveKeyDescription],
+        encryptionContext := None,
+        decryptEncryptionContext := None,
+        frameLength := Some(frameSize),
+        algorithmSuiteId := Some(algorithmSuite.id.ESDK)
+      )
+  
+  // All these tests will use a defualt CMM only Raw ECDH
+  const AllPostiveKeyringTestsNoDBESuiteNoReqECWithEphemeralRawEcdh :=
+  set
+    encryptKeyDescription <- AllRawECDH.EphemeralKeyDescriptionsEncrypt,
+    decryptKeyDescription <- AllRawECDH.DiscoveryKeyDescriptionsDecrypt | decryptKeyDescription.ECDH.curveSpec == encryptKeyDescription.ECDH.curveSpec,
+    algorithmSuite <-
+      AllAlgorithmSuites.ESDKAlgorithmSuites
+    ::
+      EsdkTestVectors.PositiveEncryptTestVectorV4(
+        encryptDescriptions := [encryptKeyDescription],
+        decryptDescriptions := [decryptKeyDescription],
+        encryptionContext := None,
+        decryptEncryptionContext := None,
+        frameLength := Some(frameSize),
+        algorithmSuiteId := Some(algorithmSuite.id.ESDK)
+      )
+  
+  const AllPostiveKeyringTestsNoDBESuiteNoReqECWithStaticRawEcdh :=
+  set
+      encryptKeyDescription <- AllRawECDH.SenderKeyDescriptions,
+      decryptKeyDescription <- AllRawECDH.RecipientKeyDescriptions | decryptKeyDescription.ECDH.curveSpec == encryptKeyDescription.ECDH.curveSpec,
+    algorithmSuite <-
+      AllAlgorithmSuites.ESDKAlgorithmSuites
+    ::
+      EsdkTestVectors.PositiveEncryptTestVectorV4(
+        encryptDescriptions := [encryptKeyDescription],
+        decryptDescriptions := [decryptKeyDescription],
+        encryptionContext := None,
+        decryptEncryptionContext := None,
+        frameLength := Some(frameSize),
+        algorithmSuiteId := Some(algorithmSuite.id.ESDK)
+      )
+  
+  const AllPostiveKeyringTestsNoDBESuiteNoReqECWithStaticDiscoveryRawEcdh :=
+  set
+      encryptKeyDescription <- AllRawECDH.SenderKeyDescriptions,
+      decryptKeyDescription <- AllRawECDH.DiscoveryKeyDescriptionsDecrypt | decryptKeyDescription.ECDH.curveSpec == encryptKeyDescription.ECDH.curveSpec,
+    algorithmSuite <-
+      AllAlgorithmSuites.ESDKAlgorithmSuites
+    ::
+      EsdkTestVectors.PositiveEncryptTestVectorV4(
+        encryptDescriptions := [encryptKeyDescription],
+        decryptDescriptions := [decryptKeyDescription],
+        encryptionContext := None,
+        decryptEncryptionContext := None,
+        frameLength := Some(frameSize),
+        algorithmSuiteId := Some(algorithmSuite.id.ESDK)
+      )
+  
+  // All these tests will use a defualt CMM only Kms ECDH
+  
+  const AllPostiveKeyringTestsNoDBESuiteNoReqECWithStaticKmsEcdh :=
+  set
+      encryptKeyDescription <- AllKmsEcdh.StaticKmsDescriptionsEncryptSender,
+      decryptKeyDescription <- AllKmsEcdh.StaticKmsDescriptionsEncryptRecipient | decryptKeyDescription.KmsECDH.curveSpec == encryptKeyDescription.KmsECDH.curveSpec,
+    algorithmSuite <-
+      AllAlgorithmSuites.ESDKAlgorithmSuites
+    ::
+      EsdkTestVectors.PositiveEncryptTestVectorV4(
+        encryptDescriptions := [encryptKeyDescription],
+        decryptDescriptions := [decryptKeyDescription],
+        encryptionContext := None,
+        decryptEncryptionContext := None,
+        frameLength := Some(frameSize),
+        algorithmSuiteId := Some(algorithmSuite.id.ESDK)
+      )
+
+  const AllPostiveKeyringTestsNoDBESuiteNoReqECWithDiscoveryKmsEcdh :=
+  set
+      encryptKeyDescription <- AllKmsEcdh.StaticKmsDescriptionsEncryptSender,
+      decryptKeyDescription <- AllKmsEcdh.DiscoveryKeyDescriptionsDecrypt | decryptKeyDescription.KmsECDH.curveSpec == encryptKeyDescription.KmsECDH.curveSpec,
+    algorithmSuite <-
+      AllAlgorithmSuites.ESDKAlgorithmSuites
+    ::
+      EsdkTestVectors.PositiveEncryptTestVectorV4(
+        encryptDescriptions := [encryptKeyDescription],
+        decryptDescriptions := [decryptKeyDescription],
+        encryptionContext := None,
+        decryptEncryptionContext := None,
+        frameLength := Some(frameSize),
+        algorithmSuiteId := Some(algorithmSuite.id.ESDK)
+      )
+    
+  
+  const Tests := 
+    AllPostiveKeyringTestsNoDBESuiteNoReqECNoEcdh + 
+    AllPostiveKeyringTestsNoDBESuiteNoReqECWithEphemeralRawEcdh +
+    AllPostiveKeyringTestsNoDBESuiteNoReqECWithStaticRawEcdh +
+    AllPostiveKeyringTestsNoDBESuiteNoReqECWithStaticDiscoveryRawEcdh +
+    AllPostiveKeyringTestsNoDBESuiteNoReqECWithStaticKmsEcdh +
+    AllPostiveKeyringTestsNoDBESuiteNoReqECWithDiscoveryKmsEcdh
+    
+}
