TestVectors/dafny/ESDK/src/VectorsComposition/AllEsdkV4WithReqEc.dfy
@@ -1,0 +1,195 @@
+// Copyright Amazon.com Inc. or its affiliates. All Rights Reserved.
+// SPDX-License-Identifier: Apache-2.0
+
+include "../LibraryIndex.dfy"
+
+module {:options "/functionSyntax:4" } AllEsdkV4WithReqEc {
+  import Types = AwsCryptographyEncryptionSdkTypes
+  import mplTypes = AwsCryptographyMaterialProvidersTypes
+  import EncryptionSdk
+  import MaterialProviders
+  import opened CompleteVectors
+  import opened KeyDescription
+  import opened Wrappers
+  import opened StandardLibrary.UInt
+  import HexStrings
+  import opened JSON.Values
+  import JSONHelpers
+  import EsdkManifestOptions
+  import EsdkTestVectors
+  import AllEsdkV4NoReqEc
+  
+  import AllHierarchy
+  import AllKms
+  import AllKmsMrkAware
+  import AllKmsMrkAwareDiscovery
+  import AllKmsRsa
+  import AllKmsEcdh
+  import AllRawAES
+  import AllRawRSA
+  import AllRawECDH
+  import AllDefaultCmm
+  import AllRequiredEncryptionContextCmm
+  import AllMulti
+
+  import UUID
+  import UTF8
+  import JSON.API
+  import SortedSets
+  import FileIO
+  
+  // This is a HACK!
+  // This is *ONLY* because this is wrapping the MPL
+  import AlgorithmSuites
+
+  datatype PositiveESDKDescriptionJSON = PositiveESDKDescriptionJSON(
+    description: string,
+    inputEncryptionContext: string,
+    requiredEncryptionContextKeys: string,
+    reproducedEncryptionContext: string,
+    encrypt: JSON,
+    decrypt: JSON
+  )
+
+  datatype SmallEncryptionContextVariation = Empty | A | AB | BA
+
+  const AllSmallEncryptionContextVariants := ["A", "AB", "BA"]
+  const RequiredEncryptionContextKeys := ["A", "B"]
+
+  const AllReqECCmmInfo :=
+    set
+      ec <- AllSmallEncryptionContextVariants,
+      requiredKeys <- RequiredEncryptionContextKeys
+      ::
+        var cmmOnEncryptDescription := Object([
+                                                ("type", String("Required Encryption Context CMM")),
+                                                ("Input Encryption Context", String(ec)),
+                                                ("Required Encryption Context Keys", String(requiredKeys))
+                                              ]);
+        var cmmOnDecryptDescription := Object([
+                                                ("type", String("Required Encryption Context CMM")),
+                                                ("Reproduced Encryption Context", String(ec)),
+                                                ("Required Encryption Context Keys", String(requiredKeys))
+                                              ]);
+        PositiveESDKDescriptionJSON(
+          description := "Generated with Required Encryption Context Keys " + requiredKeys,
+          inputEncryptionContext := ec,
+          requiredEncryptionContextKeys := requiredKeys,
+          reproducedEncryptionContext := ec,
+          encrypt := cmmOnEncryptDescription,
+          decrypt := cmmOnDecryptDescription
+        )
+  
+  const frameSize: int64 := 512
+
+
+  // All these tests will use a defualt CMM no ECDH
+  const AllPostiveKeyringTestsNoDBESuiteNoReqECNoEcdh :=
+  set
+    positiveCMMDescription <- AllReqECCmmInfo,
+    postiveKeyDescription <- AllEsdkV4NoReqEc.AllPositiveKeyDescriptions,
+    algorithmSuite <-
+      AllAlgorithmSuites.ESDKAlgorithmSuites
+    ::
+      EsdkTestVectors.PositiveEncryptTestVectorV4(
+        encryptDescriptions := [postiveKeyDescription],
+        decryptDescriptions := [postiveKeyDescription],
+        encryptionContext := None,
+        decryptEncryptionContext := None,
+        frameLength := Some(frameSize),
+        algorithmSuiteId := Some(algorithmSuite.id.ESDK)
+      )
+  
+  // // All these tests will use a defualt CMM only Raw ECDH
+  // const AllPostiveKeyringTestsNoDBESuiteNoReqECWithEphemeralRawEcdh :=
+  // set
+  //   encryptKeyDescription <- AllRawECDH.EphemeralKeyDescriptionsEncrypt,
+  //   decryptKeyDescription <- AllRawECDH.DiscoveryKeyDescriptionsDecrypt | decryptKeyDescription.ECDH.curveSpec == encryptKeyDescription.ECDH.curveSpec,
+  //   algorithmSuite <-
+  //     AllAlgorithmSuites.ESDKAlgorithmSuites
+  //   ::
+  //     EsdkTestVectors.PositiveEncryptTestVectorV4(
+  //       encryptDescriptions := [encryptKeyDescription],
+  //       decryptDescriptions := [decryptKeyDescription],
+  //       encryptionContext := None,
+  //       decryptEncryptionContext := None,
+  //       frameLength := Some(frameSize),
+  //       algorithmSuiteId := Some(algorithmSuite.id.ESDK)
+  //     )
+  
+  // const AllPostiveKeyringTestsNoDBESuiteNoReqECWithStaticRawEcdh :=
+  // set
+  //     encryptKeyDescription <- AllRawECDH.SenderKeyDescriptions,
+  //     decryptKeyDescription <- AllRawECDH.RecipientKeyDescriptions | decryptKeyDescription.ECDH.curveSpec == encryptKeyDescription.ECDH.curveSpec,
+  //   algorithmSuite <-
+  //     AllAlgorithmSuites.ESDKAlgorithmSuites
+  //   ::
+  //     EsdkTestVectors.PositiveEncryptTestVectorV4(
+  //       encryptDescriptions := [encryptKeyDescription],
+  //       decryptDescriptions := [decryptKeyDescription],
+  //       encryptionContext := None,
+  //       decryptEncryptionContext := None,
+  //       frameLength := Some(frameSize),
+  //       algorithmSuiteId := Some(algorithmSuite.id.ESDK)
+  //     )
+  
+  // const AllPostiveKeyringTestsNoDBESuiteNoReqECWithStaticDiscoveryRawEcdh :=
+  // set
+  //     encryptKeyDescription <- AllRawECDH.SenderKeyDescriptions,
+  //     decryptKeyDescription <- AllRawECDH.DiscoveryKeyDescriptionsDecrypt | decryptKeyDescription.ECDH.curveSpec == encryptKeyDescription.ECDH.curveSpec,
+  //   algorithmSuite <-
+  //     AllAlgorithmSuites.ESDKAlgorithmSuites
+  //   ::
+  //     EsdkTestVectors.PositiveEncryptTestVectorV4(
+  //       encryptDescriptions := [encryptKeyDescription],
+  //       decryptDescriptions := [decryptKeyDescription],
+  //       encryptionContext := None,
+  //       decryptEncryptionContext := None,
+  //       frameLength := Some(frameSize),
+  //       algorithmSuiteId := Some(algorithmSuite.id.ESDK)
+  //     )
+  
+  // // All these tests will use a defualt CMM only Kms ECDH
+  
+  // const AllPostiveKeyringTestsNoDBESuiteNoReqECWithStaticKmsEcdh :=
+  // set
+  //     encryptKeyDescription <- AllKmsEcdh.StaticKmsDescriptionsEncryptSender,
+  //     decryptKeyDescription <- AllKmsEcdh.StaticKmsDescriptionsEncryptRecipient | decryptKeyDescription.KmsECDH.curveSpec == encryptKeyDescription.KmsECDH.curveSpec,
+  //   algorithmSuite <-
+  //     AllAlgorithmSuites.ESDKAlgorithmSuites
+  //   ::
+  //     EsdkTestVectors.PositiveEncryptTestVectorV4(
+  //       encryptDescriptions := [encryptKeyDescription],
+  //       decryptDescriptions := [decryptKeyDescription],
+  //       encryptionContext := None,
+  //       decryptEncryptionContext := None,
+  //       frameLength := Some(frameSize),
+  //       algorithmSuiteId := Some(algorithmSuite.id.ESDK)
+  //     )
+
+  // const AllPostiveKeyringTestsNoDBESuiteNoReqECWithDiscoveryKmsEcdh :=
+  // set
+  //     encryptKeyDescription <- AllKmsEcdh.StaticKmsDescriptionsEncryptSender,
+  //     decryptKeyDescription <- AllKmsEcdh.DiscoveryKeyDescriptionsDecrypt | decryptKeyDescription.KmsECDH.curveSpec == encryptKeyDescription.KmsECDH.curveSpec,
+  //   algorithmSuite <-
+  //     AllAlgorithmSuites.ESDKAlgorithmSuites
+  //   ::
+  //     EsdkTestVectors.PositiveEncryptTestVectorV4(
+  //       encryptDescriptions := [encryptKeyDescription],
+  //       decryptDescriptions := [decryptKeyDescription],
+  //       encryptionContext := None,
+  //       decryptEncryptionContext := None,
+  //       frameLength := Some(frameSize),
+  //       algorithmSuiteId := Some(algorithmSuite.id.ESDK)
+  //     )
+    
+  
+  // const Tests := 
+  //   AllPostiveKeyringTestsNoDBESuiteNoReqECNoEcdh + 
+  //   AllPostiveKeyringTestsNoDBESuiteNoReqECWithEphemeralRawEcdh +
+  //   AllPostiveKeyringTestsNoDBESuiteNoReqECWithStaticRawEcdh +
+  //   AllPostiveKeyringTestsNoDBESuiteNoReqECWithStaticDiscoveryRawEcdh +
+  //   AllPostiveKeyringTestsNoDBESuiteNoReqECWithStaticKmsEcdh +
+  //   AllPostiveKeyringTestsNoDBESuiteNoReqECWithDiscoveryKmsEcdh
+    
+}
